iris/SpecKexecB3.v
@@ -62,6 +62,7 @@ Require Import ProcInv.
 Require Import UserPtTree.
 Require Import FileInvDefs.
 Require Import SpecKexec.
+Require Import KexecOkQ.
 Require Import SpecDirlink.
 Require Import ProofKexecSeam.
 From Kernel Require KernelSyms.
@@ -96,6 +97,7 @@ Notation Ra0 := (mword_of_int 10 : mword 5).
 (*  from ProofKexecB3.v; see that file for the design. *)
 (* ===================================================================== *)
 Definition kxc_b2_body
+      (Q : mword 64 -> Prop)
     `{!riscvGS Σ, !xv6G Σ, !bioslotG Σ, !fdslotG Σ, !fileG Σ, !irefslotG Σ, !pavG Σ} `{GEN : GenId} `{CID0 : CpuId}
     (gs : list gname) (jp : nat) (gl : gname)
     (gu : uart_names) (gd : disk_names) (gk : gname) (pd pav pu : mword 64)
@@ -145,7 +147,7 @@ Definition kxc_b2_body
     ∀ (mf : regfile) (V' : pprivate)
       (entry spv szv' : mword 64),
         ⌜callee_saved m mf⌝ -∗
-        ⌜kexec_ok V V' (mf !!! Regidx Ra0) entry spv szv' na alen⌝ -∗
+        ⌜kexec_ok_q Q V V' (mf !!! Regidx Ra0) entry spv szv' na alen⌝ -∗
         sie_cap_gpr KT1 mf K eb (proc_addr jp) -∗
         cpu_own 0 eb (proc_addr jp) eb ∅ -∗
         trap_csrs_ext KT1 eb -∗
@@ -175,7 +177,7 @@ Definition kxc_b2_body
         ∀ (mf : regfile) (V' : pprivate)
           (entry spv szv2 : mword 64),
             ⌜callee_saved m mf⌝ -∗
-            ⌜kexec_ok V V' (mf !!! Regidx Ra0) entry spv szv2 na alen⌝ -∗
+            ⌜kexec_ok_q Q V V' (mf !!! Regidx Ra0) entry spv szv2 na alen⌝ -∗
             sie_cap_gpr KT1 mf K eb (proc_addr jp) -∗
             cpu_own 0 eb (proc_addr jp) eb ∅ -∗
             trap_csrs_ext KT1 eb -∗
@@ -254,6 +256,7 @@ Definition kxc_b2z_body
 Module Type KEXECB3.
   Parameter kxc_b2 :
     forall `{!riscvGS Σ, !xv6G Σ, !bioslotG Σ, !fdslotG Σ, !fileG Σ, !irefslotG Σ, !pavG Σ} `{GEN : GenId} `{CID0 : CpuId}
+      (Q : mword 64 -> Prop)
       (gs : list gname) (jp : nat) (gl : gname)
       (gu : uart_names) (gd : disk_names) (gk : gname) (pd pav pu : mword 64)
       (bn : bio_names) (g : log_names) (gfs : fs_names) (gi : gname)
@@ -269,7 +272,7 @@ Module Type KEXECB3.
       (m M : regfile) (K : nat)
       (sp0 ra0 s00 s10 s20 pv av w67 : mword 64)
       (ef : nat -> bv 8) (P : uptd) (i : nat) (szv : mword 64),
-    kxc_b2_body gs jp gl gu gd gk pd pav pu bn g gfs gi cn gtl gilf gislf
+    kxc_b2_body Q gs jp gl gu gd gk pd pav pu bn g gfs gi cn gtl gilf gislf
       ga gf cov logstart bmapstart inodestart nib size dev
       kf qf sf gyf inumf dnf bmf n2 plen pfun na avf alen aslen afun
       pidv V eb dqb dqs dqa dqpv dqas m M K sp0 ra0 s00 s10 s20 pv av w67
